@base <http://example.org/>.
@prefix rdfs: <http://www.w3.org/2000/01/rdf-schema#> .
@prefix rdf: <http://www.w3.org/1999/02/22-rdf-syntax-ns#> .
@prefix xsd: <http://www.w3.org/2001/XMLSchema#> .
@prefix foaf: <http://xmlns.com/foaf/0.1/> .
@prefix acad: <http://acad.io/schema#> .
@prefix acaddata: <http://acad.io/data#> .
@prefix vivo: <http://vivoweb.org/ontology/core#> .

# vivo:Course was used instead------------------------------------------------------------------------------------------
# acad:Course
#   a rdfs:Class ;
#   rdfs:label "Course"@en .

acad:courseKey
    a rdf:Property ;
    rdfs:domain vivo:Course ;
    rdfs:range xsd:string ;
    rdfs:label "Course Key"@en ;
    rdfs:comment "A course key is an abstract property to uniquely identify the course."@en .

# foaf:name was used instead--------------------------------------------------------------------------------------------
#acad:courseName
#    a rdf:Property ;
#    rdfs:domain vivo:Course ;
#    rdfs:range xsd:string ;
#    rdfs:label "Course Name"@en .

acad:courseSubject
    a rdf:Property ;
    rdfs:domain vivo:Course ;
    rdfs:range xsd:string ;
    rdfs:label "Course Subject"@en ;
    rdfs:comment "A course subject is the first part of a course code and is often a series of letters, indicating the course's general subject/discipline."@en .

acad:courseNumber
    a rdf:Property ;
    rdfs:domain vivo:Course ;
    rdfs:range xsd:Integer ;
    rdfs:label "Course Number"@en ;
    rdfs:comment "A course number is the second part of a course code and is often three to four digits long. The number identifies the course level and distinguish different courses that are from the same department at the same level."@en .

# vivo:description was used instead-------------------------------------------------------------------------------------
acad:courseDescription
    a rdf:Property ;
    rdfs:domain vivo:Course ;
    rdfs:range xsd:string ;
    rdfs:label "Course Description"@en .
